switch to IsRen substs in SN proof

LeanStlc/StrongNorm.lean
@@ -14,185 +14,148 @@ abbrev SnIndices : SnVariant -> Type
 | .red => (Term) × (Term)
 
 -- TODO: prove the SN is equivalent to SN Red in LeanSubst
-inductive SN : (v : SnVariant) -> SnIndices v -> Prop where
-| var {x} : SN .neu (#x)
+inductive SNi : (v : SnVariant) -> SnIndices v -> Prop where
+| var {x} : SNi .neu (#x)
 | app {s t} :
-  SN .neu s ->
-  SN .nor t ->
-  SN .neu (s :@ t)
+  SNi .neu s ->
+  SNi .nor t ->
+  SNi .neu (s :@ t)
 | lam {t A} :
-  SN .nor t ->
-  SN .nor (:λ[A] t)
+  SNi .nor t ->
+  SNi .nor (:λ[A] t)
 | neu {t} :
-  SN .neu t ->
-  SN .nor t
+  SNi .neu t ->
+  SNi .nor t
 | red {t t'} :
-  SN .red (t, t') ->
-  SN .nor t' ->
-  SN .nor t
+  SNi .red (t, t') ->
+  SNi .nor t' ->
+  SNi .nor t
 | beta {t A b} :
-  SN .nor t ->
-  SN .red ((:λ[A] b) :@ t, b[.su t :: I])
+  SNi .nor t ->
+  SNi .red ((:λ[A] b) :@ t, b[.su t :: I])
 | step {s s' t} :
-  SN .red (s, s') ->
-  SN .red (s :@ t, s' :@ t)
+  SNi .red (s, s') ->
+  SNi .red (s :@ t, s' :@ t)
 
-namespace SN
-  -- TODO: generalize renaming lemmas to substituion of 0 size lemmas so we don't
-  -- have to mess around with the subst_var_invariant business
+namespace SNi
   @[simp]
-  abbrev SnRenameLemmaType (r : Ren) : (v : SnVariant) -> (i : SnIndices v) -> Prop
-  | .neu, t => SN .neu (t[r.to])
-  | .nor, t => SN .nor (t[r.to])
-  | .red, (t, t') => SN .red (t[r.to], t'[r.to])
+  abbrev SnRenameLemmaType (σ : Subst Term) (_ : IsRen σ) :
+    (v : SnVariant) -> (i : SnIndices v) -> Prop
+  | .neu, t => SNi .neu (t[σ])
+  | .nor, t => SNi .nor (t[σ])
+  | .red, (t, t') => SNi .red (t[σ], t'[σ])
 
-  theorem rename {v i} r : SN v i -> SnRenameLemmaType r v i := by
-    intro j; induction j generalizing r <;> simp at *
-    case var x => apply SN.var
+  theorem rename {v i} σ h : SNi v i -> SnRenameLemmaType σ h v i := by
+    intro j; induction j generalizing σ <;> simp at *
+    case var x =>
+      unfold IsRen at h
+      replace h := h x
+      cases h; case _ k h =>
+      cases h
+      case _ h => rw [h]; simp; apply SNi.var
+      case _ h => rw [h]; simp; apply SNi.var
     case app i1 i2 j1 j2 ih1 ih2 =>
-      apply SN.app <;> simp [*]
+      apply SNi.app <;> simp [*]
     case lam t A j ih =>
-      apply SN.lam
-      replace ih := ih (Ren.lift r)
-      rw [Subst.lift_lemma] at ih; simp at ih
-      apply ih
+      apply SNi.lam
+      replace ih := ih σ.lift (IsRen.lift h)
+      simp at ih; apply ih
     case neu t j ih =>
-      apply SN.neu; simp [*]
+      apply SNi.neu; simp [*]
     case red t t' j1 j2 ih1 ih2 =>
-      apply SN.red (ih1 _) (ih2 _)
+      apply SNi.red (ih1 _ h) (ih2 _ h)
     case beta t A b j ih =>
-      have lem := @SN.beta (t[r.to]) A (b[.re 0 :: r.to ∘ S]) (ih r); simp at lem
+      have lem := @SNi.beta (t[σ]) A (b[.re 0 :: σ ∘ S]) (ih σ h); simp at lem
       apply lem
     case step s s' t j ih =>
-      apply SN.step; simp [*]
+      apply SNi.step; simp [*]
 
   @[simp]
-  abbrev SnAntiRenameLemmaType (r : Ren) : (v : SnVariant) -> (i : SnIndices v) -> Prop
-  | .neu, t => ∀ z, t = z[r.to] -> SN .neu z
-  | .nor, t => ∀ z, t = z[r.to] -> SN .nor z
+  abbrev SnAntiRenameLemmaType (σ : Subst Term) (_ : IsRen σ) :
+    (v : SnVariant) -> (i : SnIndices v) -> Prop
+  | .neu, t => ∀ z, t = z[σ] -> SNi .neu z
+  | .nor, t => ∀ z, t = z[σ] -> SNi .nor z
   | .red, (t, t') =>
-    ∀ z, t = z[r.to] ->
-    ∃ z', t' = z'[r.to] ∧ SN .red (z, z')
+    ∀ z, t = z[σ] ->
+    ∃ z', t' = z'[σ] ∧ SNi .red (z, z')
 
-  theorem antirename {v i} r : SN v i -> SnAntiRenameLemmaType r v i := by
-    intro j; induction j generalizing r <;> simp at *
+  theorem antirename {v i} σ h : SNi v i -> SnAntiRenameLemmaType σ h v i := by
+    intro j; induction j generalizing σ <;> simp at *
     case var x =>
       intro z h
       cases z <;> simp at h
-      case _ y => apply SN.var
+      case _ y => apply SNi.var
     case app s t j1 j2 ih1 ih2 =>
-      intro z h; cases z <;> simp [Ren.to] at h
+      intro z h1; cases z <;> simp at h1
+      case _ x =>
+        have lem := IsRen.var_apply_forced x h; simp at lem
+        cases lem; case _ k lem =>
+        rw [lem] at h1; injection h1
       case _ u v =>
-      apply SN.app (ih1 r _ h.1) (ih2 r _ h.2)
+        apply SNi.app (ih1 σ h _ h1.1) (ih2 σ h _ h1.2)
     case lam t A j ih =>
       intro z h
       cases z <;> simp at h
-      case _ => unfold Ren.to at h; simp at h
+      case _ σr x =>
+        have lem := IsRen.var_apply_forced x σr; simp at lem
+        cases lem; case _ k lem =>
+        rw [lem] at h; injection h
       case _ A' b =>
         cases h; case _ h1 h2 =>
-        subst h1
-        apply SN.lam
-        replace ih := ih (r.lift) b
-        rw [Subst.lift_lemma] at ih; simp at ih
-        apply ih h2
+        subst h1; apply SNi.lam
+        replace ih := ih (σ.lift) (IsRen.lift h) b
+        simp at ih; apply ih h2
     case neu t j ih =>
-      intro z h
-      apply SN.neu (ih r _ h)
+      intro z h2
+      replace ih := ih σ h z h2
+      apply SNi.neu ih
     case red t t' j1 j2 ih1 ih2 =>
-      intro z h
-      have lem := ih1 r _ h
+      intro z h2
+      have lem := ih1 σ h _ h2
       cases lem; case _ z' h2 =>
-      apply SN.red h2.2
-      apply ih2 r _ h2.1
+      apply SNi.red h2.2
+      apply ih2 σ h _ h2.1
     case beta t A b j ih =>
-      intro z h
-      cases z <;> simp [Ren.to] at h
+      intro z h2
+      cases z <;> simp at h2
+      case _ x =>
+        have lem := IsRen.var_apply_forced x h; simp at lem
+        cases lem; case _ k lem =>
+        rw [lem] at h2; injection h2
       case _ u v =>
-      cases u <;> simp [Ren.to] at h
-      case _ A' u =>
-      cases h; case _ h1 h2 =>
-      cases h1; case _ h1 h3 =>
-      subst h1
-      replace ih := ih r _ h2
-      subst h2; subst h3; simp at *
-      exists (u[.su v :: I]); simp
-      apply SN.beta ih
-    case step s s' t j ih =>
-      intro z h
-      cases z <;> simp [Ren.to] at h
-      case _ u v =>
-      replace ih := ih r _ h.1
-      cases ih; case _ z' h' =>
-      exists (z' :@ v); simp [*]
-      apply SN.step (h'.2)
-
-  theorem subst_var_invariant_lift_re {σ τ : Subst Term} :
-    (∀ i k, σ i = .re k -> τ i = .re k) ->
-    (∀ i k, σ.lift i = .re k -> τ.lift i = .re k)
-  := by
-    intro h1 i k h2
-    cases i <;> simp at *; apply h2
-    case _ i =>
-      unfold Subst.compose at *; simp at *
-      generalize zdef : σ i = z at *
-      cases z <;> simp at *
-      case _ j =>
-        subst h2; rw [h1 _ _ zdef]
-
-  theorem subst_var_invariant_lift_su {σ τ : Subst Term} :
-    (∀ i t, σ i = .su t -> τ i = .su t ∨ (∃ x, t = #x ∧ τ i = .re x)) ->
-    (∀ i t, σ.lift i = .su t -> τ.lift i = .su t ∨ (∃ x, t = #x ∧ τ.lift i = .re x))
-  := by
-    intro h1 i t h2
-    cases i <;> simp at *
-    case _ i =>
-      unfold Subst.compose at *; simp at *
-      generalize zdef : σ i = z at *
-      cases z <;> simp at *
-      case _ t' =>
-        replace h1 := h1 i t' zdef
-        cases h1
-        case _ h1 =>
-          rw [h1]; simp [*]
-        case _ h1 =>
-          cases h1; case _ w h1 =>
+        cases u <;> simp at h2
+        case _ x =>
+          have lem := IsRen.var_apply_forced x h; simp at lem
+          cases lem; case _ k lem =>
+          rw [lem] at h2; injection h2.1
+        case _ A' u =>
+          cases h2; case _ h1 h2 =>
           cases h1; case _ h1 h3 =>
-          subst h1; subst h2; rw [h3]; simp
-
-  theorem subst_var_invariant {t} (σ τ : Subst Term) :
-    (∀ i k, σ i = .re k -> τ i = .re k) ->
-    (∀ i t, σ i = .su t -> τ i = .su t ∨ (∃ x, t = #x ∧ τ i = .re x)) ->
-    t[σ] = t[τ]
-  := by
-    intro h1 h2
-    induction t generalizing σ τ <;> simp
-    case var x =>
-      generalize zdef : σ x = z at *
-      cases z <;> simp
-      case _ k => rw [h1 x k zdef]
-      case _ t =>
-        have lem := h2 x t zdef
-        cases lem
-        case _ lem => rw [lem]
-        case _ lem =>
-          cases lem; case _ w lem =>
-          cases lem; case _ e lem =>
-          subst e; rw [lem]
-    case app f a ih1 ih2 =>
-      apply And.intro (ih1 _ _ h1 h2) (ih2 _ _ h1 h2)
-    case lam A t ih =>
-      replace ih := ih σ.lift τ.lift
-        (subst_var_invariant_lift_re h1)
-        (subst_var_invariant_lift_su h2)
-      simp at ih; apply ih
+          subst h1
+          replace ih := ih σ h _ h2
+          subst h2; subst h3; simp at *
+          exists (u[.su v :: I]); simp
+          apply SNi.beta ih
+    case step s s' t j ih =>
+      intro z h2
+      cases z <;> simp at h2
+      case _ x =>
+        have lem := IsRen.var_apply_forced x h; simp at lem
+        cases lem; case _ k lem =>
+        rw [lem] at h2; injection h2
+      case _ u v =>
+        replace ih := ih σ h _ h2.1
+        cases ih; case _ z' h' =>
+        exists (z' :@ v); simp [*]
+        apply SNi.step (h'.2)
 
   @[simp]
   abbrev SnBetaVarLemmaType : (v : SnVariant) -> (i : SnIndices v) -> Prop
-  | .neu, s => ∀ t x, s = t :@ #x -> SN .neu t
-  | .nor, s => ∀ t x, s = t :@ #x -> SN .nor t
+  | .neu, s => ∀ t x, s = t :@ #x -> SNi .neu t
+  | .nor, s => ∀ t x, s = t :@ #x -> SNi .nor t
   | .red, _ => True
 
-  theorem beta_var {v i} : SN v i -> SnBetaVarLemmaType v i := by
+  theorem beta_var {v i} : SNi v i -> SnBetaVarLemmaType v i := by
     intro j; induction j <;> simp at *
     case app s t j1 j2 ih1 ih2 =>
       intro u x e1 e2; subst e1; subst e2
@@ -204,7 +167,7 @@ namespace SN
       cases e; case _ e1 e2 =>
       subst e1; subst e2
       cases j; case _ j1 j2 =>
-      apply SN.neu j1
+      apply SNi.neu j1
     case red t t' j1 j2 ih1 ih2 =>
       intro u x e
       cases t <;> simp at e
@@ -213,32 +176,21 @@ namespace SN
       subst e1; subst e2
       cases j1
       case beta A b j1 =>
-        apply SN.lam
-        rw [subst_var_invariant (.su #x :: I) (.re x :: I)] at j2
-        apply @antirename .nor (b[.re x :: I]) (x :: id) j2
-        have lem : .re x :: I = @Ren.to Term (x :: id) := by
-          funext; case _ x =>
-          cases x <;> simp [Ren.to]
-        rw [lem]
-        case _ =>
-          intro i k h
-          cases i <;> simp at *
-          apply h
-        case _ =>
-          intro i t h
-          cases i <;> simp at *
-          subst h; rfl
+        apply SNi.lam
+        apply @antirename .nor (b[.su #x :: I]) (.su #x :: I) _ j2
+        rfl; unfold IsRen; intro i
+        cases i <;> simp
       case step s' j1 =>
         replace ih2 := ih2 s' x rfl
-        apply SN.red j1 ih2
+        apply SNi.red j1 ih2
 
-end SN
+end SNi
 
 namespace StrongNormalizaton
   @[simp]
   def LR : Ty -> (Term -> Prop)
-  | .base => λ t => SN .nor t
-  | .arrow A B => λ t => ∀ (r : Ren) (v : Term), LR A v -> LR B (t[r.to] :@ v)
+  | .base => λ t => SNi .nor t
+  | .arrow A B => λ t => ∀ (σ : Subst Term) (v : Term), IsRen σ -> LR A v -> LR B (t[σ] :@ v)
 
   @[simp]
   def GR : List Ty -> (Subst Term -> Prop)
@@ -249,51 +201,51 @@ namespace StrongNormalizaton
 
   notation:170 Γ:170 " ⊨s " t:170 " : " A:170 => SemanticTyping Γ t A
 
-  theorem monotone {A t} (r : Ren) : LR A t -> LR A (t[r.to]) := by
-    intro h; induction A generalizing t r
+  theorem monotone {A t} (σ : Subst Term) : IsRen σ -> LR A t -> LR A (t[σ]) := by
+    intro h1 h2; induction A generalizing t σ
     case _ =>
       simp at *
-      apply SN.rename _ h
+      apply SNi.rename σ h1 h2
     case _ A B ih1 ih2 =>
-      simp at *; intro r' v lv
-      replace h := h (r' ∘ r) v lv
-      simp at h; apply h
+      simp at *; intro σ' v σr lv
+      replace h2 := h2 (σ ∘ σ') v (IsRen.compose h1 σr) lv
+      simp at h2; apply h2
 
   theorem cr {A} :
-    (∀ t, LR A t -> SN .nor t)
-    ∧ (∀ t, SN .neu t -> LR A t)
-    ∧ (∀ t t', SN .red (t, t') -> LR A t' -> LR A t)
+    (∀ t, LR A t -> SNi .nor t)
+    ∧ (∀ t, SNi .neu t -> LR A t)
+    ∧ (∀ t t', SNi .red (t, t') -> LR A t' -> LR A t)
   := by
     induction A <;> simp at *
     case _ =>
       apply And.intro _ _
-      apply SN.neu
-      apply SN.red
+      apply SNi.neu
+      apply SNi.red
     case _ A B ih1 ih2 =>
       apply And.intro
       case _ =>
         intro t h
-        apply @SN.antirename .nor (t[S]) (λ x => x + 1) _ t rfl
-        apply @SN.beta_var .nor _ _ _ 0 rfl
-        replace h := h (λ x => x + 1) #0 (ih1.2.1 #0 SN.var); simp at h
+        apply @SNi.antirename .nor (t[S]) S IsRen.S _ t rfl
+        apply @SNi.beta_var .nor _ _ _ 0 rfl
+        replace h := h S #0 IsRen.S (ih1.2.1 #0 SNi.var); simp at h
         apply ih2.1 _ h
       case _ =>
         apply And.intro
         case _ =>
-          intro t h r v lv
+          intro t h σ v σr lv
           apply ih2.2.1
-          apply SN.app
-          apply SN.rename r h
+          apply SNi.app
+          apply SNi.rename σ σr h
           apply ih1.1 _ lv
         case _ =>
-          intro t t' h1 h2 r v lr
-          have lem1 := h2 r v lr
-          apply ih2.2.2 (t[r.to] :@ v) (t'[r.to] :@ v) _ lem1
-          replace h1 := SN.rename r h1; simp at h1
-          apply SN.step h1
+          intro t t' h1 h2 σ v σr lr
+          have lem1 := h2 σ v σr lr
+          apply ih2.2.2 (t[σ] :@ v) (t'[σ] :@ v) _ lem1
+          replace h1 := SNi.rename σ σr h1; simp at h1
+          apply SNi.step h1
 
   theorem var {A x} : LR A (#x) := by
-    apply cr.2.1; apply SN.var
+    apply cr.2.1; apply SNi.var
 
   theorem fundamental {Γ t A} : Γ ⊢ t : A -> Γ ⊨s t : A := by
     intro j; induction j
@@ -304,17 +256,17 @@ namespace StrongNormalizaton
       cases z <;> simp [*]
     case app Γ A B f a j1 j2 ih1 ih2 =>
       simp; intro σ h; simp at ih1
-      replace ih1 := ih1 σ h (λ x => x) (a[σ])
+      replace ih1 := ih1 σ h I (a[σ]) IsRen.I
       simp at ih1; apply ih1
       apply ih2 σ h
     case lam Γ A B t j ih =>
-      simp; intro σ h r v lv
-      have lem : t[.re 0::σ ∘ r.to ∘ S][.su v :: I] = t[.su v::σ ∘ r.to] := by simp
-      apply cr.2.2 _ (t[.su v::σ ∘ r.to])
-      have lem2 := @SN.beta v A (t[.re 0::σ ∘ r.to ∘ S]); simp at lem2
+      simp; intro σ h r v sr lv
+      have lem : t[.re 0::σ ∘ r ∘ S][.su v :: I] = t[.su v::σ ∘ r] := by simp
+      apply cr.2.2 _ (t[.su v::σ ∘ r])
+      have lem2 := @SNi.beta v A (t[.re 0::σ ∘ r ∘ S]); simp at lem2
       apply lem2
       apply cr.1 _ lv
-      replace ih := ih (.su v :: σ ∘ r.to)
+      replace ih := ih (.su v :: σ ∘ r)
       apply ih
       simp; intro x T j2
       cases x
@@ -328,12 +280,13 @@ namespace StrongNormalizaton
         generalize zdef : σ x = z at *
         cases z <;> simp at *
         case _ k =>
-          have lem := monotone r h; simp at lem
-          apply lem
-        case _ t => apply monotone r h
+          have lem := monotone r sr h; simp at lem
+          generalize wdef : r k = w at *
+          cases w <;> simp [*]
+        case _ t => apply monotone r sr h
 end StrongNormalizaton
 
-theorem strong_normalization {Γ t A} : Γ ⊢ t : A -> SN .nor t := by
+theorem strong_normalization {Γ t A} : Γ ⊢ t : A -> SNi .nor t := by
   intro j
   have lem1 : StrongNormalizaton.GR Γ I := by
     simp; intro x T h
